LeanSAT/Upstream/ToMathlib.lean
@@ -5,6 +5,8 @@ Authors: Wojciech Nawrocki
 -/
 
 import Mathlib.Tactic.Linarith
+import Mathlib.Data.Fintype.Basic
+import Mathlib.Data.Finset.Basic
 
 /-! Stuff that seems like it should be in std or mathlib. -/
 
@@ -39,3 +41,150 @@ theorem Int.eq_zero_of_lt_neg_iff_lt (i : Int) : (0 < -i ↔ 0 < i) → i = 0 :=
 
 instance : HAdd PNat Nat PNat where
   hAdd | ⟨a,h⟩, b => ⟨a+b, Nat.add_pos_left h _⟩
+
+/- Credit Kyle Miller, Timo Carlin-Burns, Eric Weiser for these lemmas: -/
+section Quotients
+def Quotient.toTrunc {α : Sort*} [s : Setoid α] (q : Quotient s) : Trunc { a // ⟦a⟧ = q } :=
+  Quotient.recOn q (fun a ↦ Trunc.mk ⟨a, rfl⟩) (fun _ _ _ ↦ Trunc.eq ..)
+
+def Quotient.elim {α β : Sort*} [s : Setoid α] (q : Quotient s)
+    (f : (a : α) → ⟦a⟧ = q → β) (h : ∀ a b ha hb, f a ha = f b hb)
+    : β :=
+  q.toTrunc.lift (fun x ↦ f x.val x.prop) (fun _ _ ↦ h ..)
+
+theorem Quotient.elim_mk {α β : Sort*} [s : Setoid α] (a : α)
+    (f : (b : α) → (⟦b⟧ : Quotient s) = ⟦a⟧ → β) (h : ∀ a b ha hb, f a ha = f b hb)
+  : ⟦a⟧.elim f h = f a rfl := by
+  simp [elim]
+  apply Trunc.lift_mk
+
+def Multiset.elim {α β : Type*} (s : Multiset α) (f : (L : List α) → L = s → β)
+    (h : ∀ a b ha hb, f a ha = f b hb) : β :=
+  Quotient.elim s f h
+
+theorem Multiset.elim_mk {α β : Type*} (L : List α)
+    (f : (L' : List α) → (⟦L'⟧ : Multiset α) = ⟦L⟧ → β) (h : ∀ a b ha hb, f a ha = f b hb)
+  : elim ⟦L⟧ f h = f L rfl := by
+  simp [elim]
+  apply Trunc.lift_mk
+
+theorem Multiset.elim_eq_forall {α β : Type*} {s : Multiset α} {f : (L : List α) → L = s → β} {h}
+    (motive : Prop) (hmotive : ∀ {L hL}, Multiset.elim s f h = f L hL → motive) : motive := by
+  induction s using Quotient.inductionOn with | _ L =>
+  exact hmotive rfl
+
+abbrev Finset.elim {α β : Type*} (s : Finset α) (f : (L : List α) → L = s.val → β)
+    (h : ∀ a b ha hb, f a ha = f b hb) : β :=
+  Multiset.elim s.val f h
+
+theorem Finset.elim_eq_forall {α β : Type*} {s : Finset α} {f : (L : List α) → L = s.val → β} {h}
+    (motive : Prop) (hmotive : ∀ {L hL}, Finset.elim s f h = f L hL → motive) : motive := by
+  rcases s with ⟨s,h⟩
+  induction s using Quotient.inductionOn with | _ L =>
+  exact hmotive rfl
+
+/-- Given a function over the (complete set of distinct) elements of a fintype,
+  and a proof the function is constant, produce the value of that function. -/
+def Fintype.elim_elems [Fintype V]
+      (f : (L : List V) → (∀ v, v ∈ L) → List.Nodup L → β)
+      (h : ∀ L1 h1 h11 L2 h2 h22, f L1 h1 h11 = f L2 h2 h22)
+      : β :=
+  Fintype.elems.elim
+    (fun L hL =>
+      f L
+        (by intro; rw [←Multiset.mem_coe, hL]; simp [Fintype.complete])
+        (by rw [←Multiset.coe_nodup, hL]; apply Finset.nodup))
+    (by intros; apply h)
+
+theorem Fintype.elim_elems_eq_forall [Fintype V] (f : (L : List V) → _ → _ → β) {h} {C : Prop}
+    (h' : ∀ L h1 h2, Fintype.elim_elems f h = f L h1 h2 → C)
+    : C
+  := by
+  apply Multiset.elim_eq_forall (motive := C)
+  intro L hL hM
+  apply h'
+  apply hM
+
+end Quotients
+
+theorem Finset.biUnion_union [DecidableEq α] [DecidableEq β] (s1 s2 : Finset α) (f : α → Finset β)
+  : Finset.biUnion (s1 ∪ s2) f = ((Finset.biUnion s1 f) ∪ Finset.biUnion s2 f)
+  := by
+  ext b
+  simp only [mem_biUnion, mem_union]
+  constructor
+  · rintro ⟨a,b|b⟩
+    · refine Or.inl ⟨a,?_⟩
+      simp only [and_self, *]
+    · refine Or.inr ⟨a,?_⟩
+      simp only [and_self, *]
+  · rintro (⟨a,b,c⟩|⟨a,b,c⟩)
+      <;> refine ⟨a, ?_⟩
+    · simp only [and_self, true_or, *]
+    · simp only [and_self, or_true, *]
+
+def Finset.getUnique (xs : Finset α) (h : ∃ x, xs = {x}) : α :=
+  xs.elim (fun L hL =>
+    match L with
+    | [] => by
+      exfalso; cases h; simp_all
+      apply Multiset.not_mem_zero
+      rw [hL]
+      apply Multiset.mem_singleton.mpr
+      rfl
+    | x::_ => x
+    ) (by
+    intro a b ha hb
+    rcases h with ⟨x,rfl⟩
+    simp at ha hb
+    cases ha; cases hb
+    simp)
+
+@[simp] theorem Finset.getUnique_eq (xs : Finset α) (h) (v)
+  : Finset.getUnique xs h = v ↔ xs = {v}
+  := by
+  rcases h with ⟨x,rfl⟩
+  simp [getUnique]
+  apply elim_eq_forall
+  intro L hL heq
+  rw [heq]; clear heq
+  simp at hL; cases hL
+  simp
+
+theorem List.Perm.find?_unique {f : α → Bool}
+    (hunique : ∀ a1 a2, f a1 → f a2 → a1 = a2) (h : a ~ b)
+  : a.find? f = b.find? f := by
+  induction h with
+  | nil => simp
+  | cons => simp [find?]; split <;> simp [*]
+  | swap =>
+    simp [find?]; split <;> split <;> simp
+    apply hunique; repeat assumption
+  | trans =>
+    simp_all
+
+def Multiset.find? (f : α → Bool) (xs : Multiset α)
+      (h : ∀ a1 a2, f a1 = true → f a2 = true → a1 = a2) : Option α :=
+  xs.lift (·.find? f) (by
+    intro a b perm
+    simp
+    apply perm.find?_unique h
+  )
+
+theorem Multiset.mem_of_find?_eq_some (xs : Multiset α)
+  : xs.find? f h = some x → x ∈ xs := by
+  have ⟨L,hL⟩ := xs.exists_rep; cases hL
+  simp [-quot_mk_to_coe, find?]
+  simp; apply List.mem_of_find?_eq_some
+
+theorem Multiset.find?_some (xs : Multiset α)
+  : xs.find? f h = some x → f x := by
+  have ⟨L,hL⟩ := xs.exists_rep; cases hL
+  simp [-quot_mk_to_coe, find?]
+  apply List.find?_some
+
+@[simp] theorem Multiset.find?_eq_none (xs : Multiset α)
+  : xs.find? f h = none ↔ ∀ x ∈ xs, f x = false := by
+  have ⟨L,hL⟩ := xs.exists_rep; cases hL
+  simp only [find?, Quotient.lift_mk, List.find?_eq_none, Bool.not_eq_true]
+  simp only [quot_mk_to_coe, mem_coe]
